assembler/RelocBingenproof.v
@@ -7,7 +7,7 @@ Require Import EncDecRet RelocBingen RelocBinDecode.
 Require Import RelocProgSemantics RelocProgSemantics1 RelocProgSemanticsArchi1.
 Require Import TranslateInstr RelocProgSemantics2.
 Require Import RelocBingenproofArchi RelocProgGlobalenvs.
-
+Require Import LocalLib.
 
 Import ListNotations.
 Local Open Scope error_monad_scope.
@@ -28,28 +28,6 @@ Proof.
     rewrite PTree.gmap in H.
     unfold option_map in *. destr_in H.
     exists a. inv H. auto.
-Qed.
-
-Lemma list_forall2_Forall2: forall A B (P: A -> B -> Prop) l1 l2,
-    list_forall2 P l1 l2 <->
-    Forall2 P l1 l2.
-Proof.
-  induction l1;intros.
-  split;intros. inv H. auto.
-  inv H. constructor.
-  split;intros.
-  inv H. constructor. auto. apply IHl1. auto.
-  inv H. constructor. auto. apply IHl1. auto.
-Qed.
-
-Lemma list_forall2_app_inv_l: forall A B (P: A -> B -> Prop) l1 l2 l3,
-    list_forall2 P (l1++l2) l3 ->
-    exists l4 l5, l3 = l4 ++ l5 /\ list_forall2 P l1 l4 /\ list_forall2 P l2 l5.
-  intros.
-  apply list_forall2_Forall2 in H.
-  exploit Forall2_app_inv_l;eauto. intros (l1' & l2' & ? & ? & ?).
-  eexists. eexists. split;eauto.
-  split;apply list_forall2_Forall2;auto.
 Qed.
 
   
