x86/RelocProgSemanticsArchi1.v
@@ -12,135 +12,135 @@ Definition rev_id_eliminate (symb: ident) (i:instruction) :=
    match i with
   | Pjmp_l_rel _ =>
      (Pjmp_s symb signature_main)
-  | Pjmp_m (Addrmode rb ss (inr disp)) =>
-    let '(id, ptrofs) := disp in
+  | Pjmp_m (Addrmode rb ss (inl disp)) =>
+    let ptrofs := Ptrofs.repr disp in
      (Pjmp_m (Addrmode rb ss (inr (symb,ptrofs))))
   | Pcall_s id sg =>
      (Pcall_s symb sg)
   | Pmov_rs rd id =>
      (Pmov_rs rd symb)
-  | Pmovl_rm rd (Addrmode rb ss (inr disp)) =>
-    let '(id, ptrofs) := disp in
+  | Pmovl_rm rd (Addrmode rb ss (inl disp)) =>
+    let ptrofs := Ptrofs.repr disp in
      (Pmovl_rm rd (Addrmode rb ss (inr (symb,ptrofs))))
-  | Pmovl_mr (Addrmode rb ss (inr disp)) rs =>
-    let '(id, ptrofs) := disp in
+  | Pmovl_mr (Addrmode rb ss (inl disp)) rs =>
+    let ptrofs := Ptrofs.repr disp in
      (Pmovl_mr (Addrmode rb ss (inr (symb, ptrofs))) rs)
-  | Pfldl_m (Addrmode rb ss (inr disp)) =>
-    let '(id, ptrofs) := disp in
+  | Pfldl_m (Addrmode rb ss (inl disp)) =>
+    let ptrofs := Ptrofs.repr disp in
      (Pfldl_m (Addrmode rb ss (inr (symb, ptrofs))))
-  | Pfstpl_m (Addrmode rb ss (inr disp)) =>
-    let '(id, ptrofs) := disp in
+  | Pfstpl_m (Addrmode rb ss (inl disp)) =>
+    let ptrofs := Ptrofs.repr disp in
      (Pfstpl_m (Addrmode rb ss (inr (symb, ptrofs))))
-  | Pflds_m (Addrmode rb ss (inr disp)) =>
-    let '(id, ptrofs) := disp in
+  | Pflds_m (Addrmode rb ss (inl disp)) =>
+    let ptrofs := Ptrofs.repr disp in
      (Pflds_m (Addrmode rb ss (inr (symb, ptrofs))))
-  | Pfstps_m (Addrmode rb ss (inr disp)) =>
-    let '(id, ptrofs) := disp in
+  | Pfstps_m (Addrmode rb ss (inl disp)) =>
+    let ptrofs := Ptrofs.repr disp in
      (Pfstps_m (Addrmode rb ss (inr (symb, ptrofs))))
-  | Pmovsd_fm rd (Addrmode rb ss (inr disp)) =>
-    let '(id, ptrofs) := disp in
+  | Pmovsd_fm rd (Addrmode rb ss (inl disp)) =>
+    let ptrofs := Ptrofs.repr disp in
      (Pmovsd_fm rd (Addrmode rb ss (inr (symb, ptrofs))))
-  | Pmovsd_mf (Addrmode rb ss (inr disp)) rs =>
-    let '(id, ptrofs) := disp in
+  | Pmovsd_mf (Addrmode rb ss (inl disp)) rs =>
+    let ptrofs := Ptrofs.repr disp in
     (Pmovsd_mf (Addrmode rb ss (inr (symb, ptrofs))) rs)
-  | Pmovsd_fm_a rd (Addrmode rb ss (inr disp)) =>
-    let '(id, ptrofs) := disp in
+  | Pmovsd_fm_a rd (Addrmode rb ss (inl disp)) =>
+    let ptrofs := Ptrofs.repr disp in
     (Pmovsd_fm rd (Addrmode rb ss (inr (symb, ptrofs))))
-  | Pmovsd_mf_a (Addrmode rb ss (inr disp)) rs =>
-    let '(id, ptrofs) := disp in
+  | Pmovsd_mf_a (Addrmode rb ss (inl disp)) rs =>
+    let ptrofs := Ptrofs.repr disp in
      (Pmovsd_mf (Addrmode rb ss (inr (symb, ptrofs))) rs)  
-  | Pmovss_fm rd (Addrmode rb ss (inr disp)) =>
-    let '(id, ptrofs) := disp in
+  | Pmovss_fm rd (Addrmode rb ss (inl disp)) =>
+    let ptrofs := Ptrofs.repr disp in
      (Pmovss_fm rd (Addrmode rb ss (inr (symb, ptrofs))))
-  | Pmovss_mf (Addrmode rb ss (inr disp)) rs =>
-    let '(id, ptrofs) := disp in
+  | Pmovss_mf (Addrmode rb ss (inl disp)) rs =>
+    let ptrofs := Ptrofs.repr disp in
      (Pmovss_mf (Addrmode rb ss (inr (symb, ptrofs))) rs)
-  | Pxorpd_fm rd (Addrmode rb ss (inr disp)) =>
-    let '(id, ptrofs) := disp in
+  | Pxorpd_fm rd (Addrmode rb ss (inl disp)) =>
+    let ptrofs := Ptrofs.repr disp in
      (Pxorpd_fm rd (Addrmode rb ss (inr (symb, ptrofs))))
-  | Pxorps_fm rd (Addrmode rb ss (inr disp)) =>
-    let '(id, ptrofs) := disp in
+  | Pxorps_fm rd (Addrmode rb ss (inl disp)) =>
+    let ptrofs := Ptrofs.repr disp in
      (Pxorps_fm rd (Addrmode rb ss (inr (symb, ptrofs))))
-  | Pandpd_fm rd (Addrmode rb ss (inr disp)) =>
-    let '(id, ptrofs) := disp in
+  | Pandpd_fm rd (Addrmode rb ss (inl disp)) =>
+    let ptrofs := Ptrofs.repr disp in
      (Pandpd_fm rd (Addrmode rb ss (inr (symb, ptrofs))))
-  | Pandps_fm rd (Addrmode rb ss (inr disp)) =>
-    let '(id, ptrofs) := disp in
+  | Pandps_fm rd (Addrmode rb ss (inl disp)) =>
+    let ptrofs := Ptrofs.repr disp in
      (Pandps_fm rd (Addrmode rb ss (inr (symb, ptrofs))))
   (** Moves with conversion *)
-  | Pmovb_mr (Addrmode rb ss (inr disp)) rs =>
-    let '(id, ptrofs) := disp in
+  | Pmovb_mr (Addrmode rb ss (inl disp)) rs =>
+    let ptrofs := Ptrofs.repr disp in
      (Pmovb_mr (Addrmode rb ss (inr (symb, ptrofs))) rs)
-  | Pmovb_rm rd (Addrmode rb ss (inr disp)) =>
-    let '(id, ptrofs) := disp in
+  | Pmovb_rm rd (Addrmode rb ss (inl disp)) =>
+    let ptrofs := Ptrofs.repr disp in
      (Pmovb_rm rd (Addrmode rb ss (inr (symb, ptrofs))))
-  | Pmovw_mr (Addrmode rb ss (inr disp)) rs =>
-    let '(id, ptrofs) := disp in
+  | Pmovw_mr (Addrmode rb ss (inl disp)) rs =>
+    let ptrofs := Ptrofs.repr disp in
      (Pmovw_mr (Addrmode rb ss (inr (symb, ptrofs))) rs)
-  | Pmovw_rm rd (Addrmode rb ss (inr disp)) =>
-    let '(id, ptrofs) := disp in
+  | Pmovw_rm rd (Addrmode rb ss (inl disp)) =>
+    let ptrofs := Ptrofs.repr disp in
      (Pmovw_rm rd (Addrmode rb ss (inr (symb, ptrofs))))
-  | Pmovzb_rm rd (Addrmode rb ss (inr disp)) =>
-    let '(id, ptrofs) := disp in
+  | Pmovzb_rm rd (Addrmode rb ss (inl disp)) =>
+    let ptrofs := Ptrofs.repr disp in
      (Pmovzb_rm rd (Addrmode rb ss (inr (symb, ptrofs))))
-  | Pmovsb_rm rd (Addrmode rb ss (inr disp)) =>
-    let '(id, ptrofs) := disp in
+  | Pmovsb_rm rd (Addrmode rb ss (inl disp)) =>
+    let ptrofs := Ptrofs.repr disp in
      (Pmovsb_rm rd (Addrmode rb ss (inr (symb, ptrofs))))
-  | Pmovzw_rm rd (Addrmode rb ss (inr disp)) =>
-    let '(id, ptrofs) := disp in
+  | Pmovzw_rm rd (Addrmode rb ss (inl disp)) =>
+    let ptrofs := Ptrofs.repr disp in
      (Pmovzw_rm rd (Addrmode rb ss (inr (symb, ptrofs))))
-  | Pmovsw_rm rd (Addrmode rb ss (inr disp)) =>
-    let '(id, ptrofs) := disp in
+  | Pmovsw_rm rd (Addrmode rb ss (inl disp)) =>
+    let ptrofs := Ptrofs.repr disp in
      (Pmovsw_rm rd (Addrmode rb ss (inr (symb, ptrofs))))
-  | Pmovsq_rm rd (Addrmode rb ss (inr disp)) =>
-    let '(id, ptrofs) := disp in
+  | Pmovsq_rm rd (Addrmode rb ss (inl disp)) =>
+    let ptrofs := Ptrofs.repr disp in
      (Pmovsq_rm rd (Addrmode rb ss (inr (symb, ptrofs))))
-  | Pmovsq_mr (Addrmode rb ss (inr disp)) rs =>
-    let '(id, ptrofs) := disp in
+  | Pmovsq_mr (Addrmode rb ss (inl disp)) rs =>
+    let ptrofs := Ptrofs.repr disp in
      (Pmovsq_mr (Addrmode rb ss (inr (symb, ptrofs))) rs)
   (** Integer arithmetic *)
-  | Pleal rd (Addrmode rb ss (inr disp))  =>
-    let '(id, ptrofs) := disp in
+  | Pleal rd (Addrmode rb ss (inl disp))  =>
+    let ptrofs := Ptrofs.repr disp in
      (Pleal rd (Addrmode rb ss (inr (symb, ptrofs))))
   (** Saving and restoring registers *)
-  | Pmov_rm_a rd (Addrmode rb ss (inr disp)) =>  (**r like [Pmov_rm], using [Many64] chunk *)
-    let '(id, ptrofs) := disp in
+  | Pmov_rm_a rd (Addrmode rb ss (inl disp)) =>  (**r like [Pmov_rm], using [Many64] chunk *)
+    let ptrofs := Ptrofs.repr disp in
      (Pmov_rm_a rd (Addrmode rb ss (inr (symb, ptrofs))))
-  | Pmov_mr_a (Addrmode rb ss (inr disp)) rs =>   (**r like [Pmov_mr], using [Many64] chunk *)
-    let '(id, ptrofs) := disp in
+  | Pmov_mr_a (Addrmode rb ss (inl disp)) rs =>   (**r like [Pmov_mr], using [Many64] chunk *)
+    let ptrofs := Ptrofs.repr disp in
     (Pmov_mr_a (Addrmode rb ss (inr (symb, ptrofs))) rs)
-  | Paddq_rm rd (Addrmode rb ss (inr disp))  =>
-    let '(id, ptrofs) := disp in
+  | Paddq_rm rd (Addrmode rb ss (inl disp))  =>
+    let ptrofs := Ptrofs.repr disp in
     (Paddq_rm rd (Addrmode rb ss (inr (symb, ptrofs))))
-  | Psubq_rm rd (Addrmode rb ss (inr disp))  =>
-    let '(id, ptrofs) := disp in
+  | Psubq_rm rd (Addrmode rb ss (inl disp))  =>
+    let ptrofs := Ptrofs.repr disp in
     (Psubq_rm rd (Addrmode rb ss (inr (symb, ptrofs))))
-  | Pimulq_rm rd (Addrmode rb ss (inr disp))  =>
-    let '(id, ptrofs) := disp in
+  | Pimulq_rm rd (Addrmode rb ss (inl disp))  =>
+    let ptrofs := Ptrofs.repr disp in
     (Pimulq_rm rd (Addrmode rb ss (inr (symb, ptrofs))))
-  | Pandq_rm rd (Addrmode rb ss (inr disp))  =>
-    let '(id, ptrofs) := disp in
+  | Pandq_rm rd (Addrmode rb ss (inl disp))  =>
+    let ptrofs := Ptrofs.repr disp in
     (Pandq_rm rd (Addrmode rb ss (inr (symb, ptrofs))))
-  | Porq_rm rd (Addrmode rb ss (inr disp))  =>
-    let '(id, ptrofs) := disp in
+  | Porq_rm rd (Addrmode rb ss (inl disp))  =>
+    let ptrofs := Ptrofs.repr disp in
     (Porq_rm rd (Addrmode rb ss (inr (symb, ptrofs))))
-  | Pxorq_rm rd (Addrmode rb ss (inr disp))  =>
-    let '(id, ptrofs) := disp in
+  | Pxorq_rm rd (Addrmode rb ss (inl disp))  =>
+    let ptrofs := Ptrofs.repr disp in
     (Pxorq_rm rd (Addrmode rb ss (inr (symb, ptrofs))))
-  | Pcmpq_rm rd (Addrmode rb ss (inr disp))  =>
-    let '(id, ptrofs) := disp in
+  | Pcmpq_rm rd (Addrmode rb ss (inl disp))  =>
+    let ptrofs := Ptrofs.repr disp in
     (Pcmpq_rm rd (Addrmode rb ss (inr (symb, ptrofs))))
-  | Ptestq_rm rd (Addrmode rb ss (inr disp))  =>
-    let '(id, ptrofs) := disp in
+  | Ptestq_rm rd (Addrmode rb ss (inl disp))  =>
+    let ptrofs := Ptrofs.repr disp in
     (Ptestq_rm rd (Addrmode rb ss (inr (symb, ptrofs))))
-  | Pmovq_rm rd (Addrmode rb ss (inr disp))  =>
-    let '(id, ptrofs) := disp in
+  | Pmovq_rm rd (Addrmode rb ss (inl disp))  =>
+    let ptrofs := Ptrofs.repr disp in
     (Pmovq_rm rd (Addrmode rb ss (inr (symb, ptrofs))))
-  | Pmovq_mr (Addrmode rb ss (inr disp)) rs =>
-    let '(id, ptrofs) := disp in
+  | Pmovq_mr (Addrmode rb ss (inl disp)) rs =>
+    let ptrofs := Ptrofs.repr disp in
     (Pmovq_mr (Addrmode rb ss (inr (symb, ptrofs))) rs)
-  | Pleaq rd (Addrmode rb ss (inr disp))  =>
-    let '(id, ptrofs) := disp in
+  | Pleaq rd (Addrmode rb ss (inl disp))  =>
+    let ptrofs := Ptrofs.repr disp in
      (Pleaq rd (Addrmode rb ss (inr (symb, ptrofs))))
   | _ =>
      i
